src/examples/resource_exchange.v
@@ -1,0 +1,634 @@
+From Equations Require Import Equations.
+From iris.proofmode Require Import proofmode monpred.
+From iris.algebra Require Import gmap_view.
+From iris_named_props Require Import named_props.
+From nextgen Require Import cmra_morphism_extra gmap_view_transformation.
+
+From self Require Import extra solve_view_le encode_relation map_extra view_slice.
+
+From self.lang Require Import syntax tactics lemmas.
+
+From self.base Require Import generational_resources primitive_laws.
+
+From self.high Require Import wrappers monpred_simpl protocol locations crash_weakestpre weakestpre.
+From self.high.modalities Require Import post_fence_sync_advanced.
+From self.high.lib Require Import abstract_state increasing_map.
+From self.high Require Import weakestpre_at weakestpre_exp proofmode.
+
+From self Require Export lang.
+From self.high Require Export dprop.
+
+Set Default Proof Using "Type*".
+
+Section Program.
+    Definition try_push: expr :=
+    λ: "ℓ" "v",
+      if: Snd (CmpXchg "ℓ" NONEV (SOME "v")) then
+        #()
+      else
+        #().
+
+  Definition try_pop: expr :=
+    λ: "ℓ",
+      match: !_AT "ℓ" with
+        NONE => NONEV
+      | SOME "v" =>
+          if: Snd (CmpXchg "ℓ" (SOME "v") NONEV) then
+            Flush "ℓ";; FenceSync ;; SOME "v"
+          else
+            NONEV
+      end.
+End Program.
+
+(* The exclusive ghost resource: [gset_disj nat]. *)
+Definition excl_opsR : cmra := gmap_viewR nat unitO.
+Class excl_opsG (Σ: gFunctors) (Ω: gGenCmras Σ) := {
+  excl_ops_inG :: genInDepsG Σ Ω excl_opsR [#];
+}.
+Section Ghosts.
+  Context `{!excl_opsG Σ Ω}.
+
+  Definition drop_op (p: nat) n (_: unit): option _ :=
+    if decide (n < p) then Some () else None.
+
+  #[export] Instance drop_op_maptrans p: MapTrans (drop_op p).
+  Proof.
+    split; last solve_proper. unfold drop_above_hist.
+    intros. done.
+  Qed.
+  
+  Definition excl_ops_trans (p: nat): excl_opsR → excl_opsR :=
+    map_entry_lift_gmap_view (drop_op p).
+
+  Definition excl_ops_pred (p: nat): pred_over excl_opsR :=
+    λ t, ∃ p', p ≤ p' ∧ t = excl_ops_trans p'.
+  
+  Definition ops_auth γ (n: nat): iProp Σ :=
+    gen_own γ (gmap_view_auth (DfracOwn 1) (map_seq 0 (repeat () n))).
+
+  Definition ops_frag γ (n: nat): iProp Σ :=
+    "frag" ∷ gen_own γ (gmap_view_frag n (DfracOwn 1) ()) ∗
+    "#frag_rely_self" ∷ ∃ p', ⌜ n < p' ⌝ ∗ rely_self γ (excl_ops_pred p').
+
+  Definition ops_token γ (p: nat) :=
+    token γ [#] (excl_ops_pred p) (excl_ops_pred p).
+  
+  Lemma excl_ops_alloc:
+    ⊢ |==> ∃ γ, ops_auth γ 0 ∗ ops_token γ 0.
+  Proof.
+    iMod (own_gen_alloc (DS := [#]) (gmap_view_auth (DfracOwn 1) ∅) [#] [##] with "[]") as (γ) "(HO & tok)".
+    { by apply gmap_view_auth_valid. }
+    { iIntros (i'). inversion i'. }
+    iMod (token_strengthen_promise (DS := [#])
+            _ [#] [##] _ (excl_ops_pred 0) _ (excl_ops_pred 0) with "[] tok")
+      as "tok".
+    { intros ???. unfold True_rel. rewrite huncurry_curry. done. }
+    { done. }
+    { intros ts. dependent elimination ts. done. }
+    { intros ts _. dependent elimination ts.
+      exists (excl_ops_trans 0).
+      split; first apply _.
+      eexists.
+      done. }
+    { iIntros (i'). inversion i'. }
+    iModIntro.
+    iDestruct (token_to_rely with "tok") as "#rely".
+    iDestruct (rely_to_rely_self with "rely") as "?".
+    iExists _.
+    iFrame "∗#".
+  Qed.
+  
+  #[export] Instance ops_frag_into_base_nextgen {γ} n:
+    base_IntoNextgen
+      (ops_frag γ n)
+      (ops_frag γ n).
+  Proof.
+    rewrite /base_IntoNextgen /ops_frag.
+    iNamed 1.
+    iModIntro.
+    iDestruct "frag" as (t) "[picked_in frag]".
+    iDestruct "frag_rely_self" as (p Hlt) "[rely_self (%t' & (%p' & %Hle & %H) & picked_in')]".
+    iPickedInAgree "picked_in picked_in'".
+    subst t.
+    iSplitL "frag".
+    { iApply (gen_own_proper with "frag").
+      rewrite /excl_ops_trans.
+      unfold map_entry_lift_gmap_view, gMapTrans_frag_lift, map_trans_frag_lift, fmap_view, fmap_pair. simpl.
+      unfold gmap_view_frag, view_frag.
+      f_equiv.
+      rewrite -{2}insert_empty.
+      erewrite map_imap_insert_Some;
+        first rewrite map_imap_empty insert_empty //.
+      rewrite agree_option_map_to_agree /drop_op decide_True //.
+      lia. }
+    iExists p.
+    by iFrame "#".
+  Qed.
+
+  Lemma map_seq_grow (n: nat):
+    (map_seq 0 (repeat () (S n)): gmap nat unit) = <[ n := () ]> (map_seq 0 (repeat () n)).
+  Proof.
+    simpl repeat.
+    rewrite repeat_cons map_seq_snoc.
+    f_equiv.
+    rewrite repeat_length //.
+  Qed.
+  
+  Lemma ops_auth_grow {γ n}:
+    ops_auth γ n ==∗ ops_auth γ (S n) ∗ gen_own γ (gmap_view_frag n (DfracOwn 1) ()).
+  Proof.
+    iIntros "ops_auth".
+    iMod (gen_own_update with "ops_auth") as "[$ $]"; last done.
+    rewrite map_seq_grow.
+    apply gmap_view_alloc; last done.
+    rewrite lookup_map_seq_0 lookup_ge_None repeat_length //.
+  Qed.
+    
+  Lemma ops_auth_ops_frag_false {γ} n:
+    ops_auth γ n -∗
+    ops_frag γ n -∗
+    False.
+  Proof.
+    iIntros "auth". iNamed 1.
+    iDestruct (gen_own_valid_2 with "auth frag") as %[_ contra]%gmap_view_both_valid_L.
+    rewrite lookup_map_seq_0 in contra.
+    apply lookup_lt_Some in contra.
+    rewrite repeat_length in contra.
+    lia.
+  Qed.
+
+  Lemma ops_token_strengthen {γ p} p':
+    p ≤ p' →
+    ops_token γ p ==∗ ops_token γ p' ∗ rely_self γ (excl_ops_pred p').
+  Proof.
+    iIntros (?) "token".
+    iMod (token_strengthen_promise_0_deps _ _ (excl_ops_pred p') with "token") as "token".
+    { rewrite /excl_ops_pred.
+      intros ? (p'' & ? & ->).
+      eexists.
+      split; last done.
+      lia. }
+    { exists (excl_ops_trans p').
+      split; first apply _.
+      by eexists. }
+    iDestruct (token_to_rely with "token") as "#rely".
+    iDestruct (rely_to_rely_self with "rely") as "$".
+    done.
+  Qed.
+
+  Lemma map_entry_lift_gmap_view_auth dq (m: gmap nat unit) map_entry :
+    (map_entry_lift_gmap_view map_entry (gmap_view_auth dq m)) =
+    (gmap_view_auth dq (map_imap map_entry m)).
+  Proof.
+    unfold map_entry_lift_gmap_view, fmap_view, fmap_pair. simpl.
+    rewrite agree_map_to_agree. done.
+  Qed.
+End Ghosts.
+Opaque ops_frag.
+
+(* We now define the abstract state used for the location [ℓ] *)
+Section Protocol.
+  Context `{!excl_opsG Σ Ω, !nvmBaseGS Σ Ω}.
+  Variables (γ: gname) (R: val → dProp Σ).
+  Hypothesis (R_buffer_free: ∀ v, BufferFree (R v)).
+  Hypothesis (R_NGF: ∀ v, IntoNGFlush (R v) (R v)).
+  #[local] Existing Instances R_buffer_free R_NGF.
+  
+  Instance list_abstract_state T `{!EqDecision T, Countable T} : AbstractState (list T) :=
+    { abs_state_relation := prefix }.
+
+  (* [inl] is push, [inr] is pop. *)
+  Notation ST := (list (val + unit)).
+
+  Definition p_pure (σ: ST) (v: val): dProp Σ :=
+    ⌜ match last σ with
+      | Some (inl w) =>
+          v = SOMEV w 
+      | _ =>  v = NONEV 
+      end ⌝.
+  
+  Definition p_full (σ: ST) (v: val): dProp Σ :=
+    ⎡ ops_auth γ (length σ) ⎤ ∗
+    match last σ with
+    | Some (inl w) => ⌜ v = SOMEV w ⌝ ∗ ⌜ val_is_unboxed v ⌝ ∗ R w
+    | _ => ⌜ v = NONEV ⌝
+    end.
+
+  Definition p_read (σ: ST) (v: val): dProp Σ :=
+    match last σ with
+    | Some (inl w) =>
+        ⌜ v = SOMEV w ⌝ ∗ ⌜ val_is_unboxed v ⌝ ∗
+        ((R w) ∨ ⎡ ops_frag γ (length σ) ⎤)
+    | _ => ⌜ v = NONEV ⌝
+    end.
+  
+  Definition p_pers (σ: ST) (v: val): dProp Σ :=
+    ⎡ ops_token γ (length σ) ⎤ ∗ p_pure σ v.
+  
+  Lemma p_read_p_pure (σ: ST) (v: val):
+    p_read σ v -∗ p_pure σ v.
+  Proof.
+    rewrite /p_read /p_pure.
+    destruct (last σ) as [[] | ]; try naive_solver.
+    iIntros "[$ _]".
+  Qed.
+  
+  Definition prot : LocationProtocol ST :=
+  {| protocol.p_full := p_full;
+     protocol.p_read := p_read;
+     protocol.p_pers := p_pers;
+     p_bumper h := h |}.
+  
+  #[export] Instance prot_cond : ProtocolConditions prot.
+  Proof.
+    split; try done; try solve_proper; try apply _.
+    - intros σ v.
+      rewrite /prot /p_full /=.
+      destruct (last σ) as [[] | ]; try apply _.
+    - intros σ v.
+      rewrite /prot /p_read /=.
+      destruct (last σ) as [[] | ]; try apply _.
+    - intros σ v.
+      apply bi.equiv_entails. split.
+      + rewrite /prot /p_full /p_read /=.
+        iIntros "[ops_auth R]".
+        iSplitL "R"; destruct (last σ) as [[ w | ] | ]; try naive_solver.
+        * iDestruct "R" as "($ & $ & R)".
+          by iLeft.
+        * iIntros "($ & $ & [ $ | ops_frag ])"; first done.
+          iDestruct (ops_auth_ops_frag_false with "ops_auth ops_frag") as %[].
+      + iIntros "[? H]".
+        by iApply "H".
+    - rewrite /prot /p_full /p_read /p_pers /p_pure /=.
+      iIntros (σ_p v_p σ_f v_f) "%HorderPF [ops_token Hσ_p] [ops_auth R]".
+      iSplit.
+      + (* we pick [t] to be [excl_ops_trans (length σ_f)] *)
+        iMod (ops_token_strengthen (length σ_f) with "ops_token") as "[ops_token _]".
+        { by apply prefix_length. }
+        iMod (token_pick (DS := [#]) _ [#] _ _ [##]%HV (excl_ops_trans (length σ_f)) with "[] ops_token") as "[token picked_out]".
+        { by eexists. }
+        { iIntros (i'). inversion i'. }
+        iModIntro.
+        (* It's difficult to get [match .. with] to work with typeclasses. *)
+        destruct (last σ_f) as [[ w | ] | ]; iModIntro.
+        * iDestruct "ops_auth" as (?) "[picked_in ops_auth]".
+          iPickedInAgree "picked_out picked_in".
+          iDestruct "R" as "[% R]".
+          iFrame "∗%".
+          rewrite /excl_ops_trans map_entry_lift_gmap_view_auth /=.
+          iApply (gen_own_proper with "ops_auth").
+          f_equiv.
+          rewrite map_equiv_iff.
+          intros i.
+          rewrite map_lookup_imap ?lookup_map_seq_0 /drop_op /=.
+          destruct (decide _); destruct (repeat () (length σ_f) !! i) as [ [] | ] eqn:Hlook; rewrite Hlook /= //.
+          apply lookup_lt_Some in Hlook.
+          rewrite repeat_length in Hlook.
+          lia.
+        * iDestruct "ops_auth" as (?) "[picked_in ops_auth]".
+          iPickedInAgree "picked_out picked_in".
+          iDestruct "R" as "%".
+          iFrame "∗%".
+          rewrite /excl_ops_trans map_entry_lift_gmap_view_auth /=.
+          iApply (gen_own_proper with "ops_auth").
+          f_equiv.
+          rewrite map_equiv_iff.
+          intros i.
+          rewrite map_lookup_imap ?lookup_map_seq_0 /drop_op /=.
+          destruct (decide _); destruct (repeat () (length σ_f) !! i) as [ [] | ] eqn:Hlook; rewrite Hlook /= //.
+          apply lookup_lt_Some in Hlook.
+          rewrite repeat_length in Hlook.
+          lia.
+        * iDestruct "ops_auth" as (?) "[picked_in ops_auth]".
+          iPickedInAgree "picked_out picked_in".
+          iDestruct "R" as "%".
+          iFrame "∗%".
+          rewrite /excl_ops_trans map_entry_lift_gmap_view_auth /=.
+          iApply (gen_own_proper with "ops_auth").
+          f_equiv.
+          rewrite map_equiv_iff.
+          intros i.
+          rewrite map_lookup_imap ?lookup_map_seq_0 /drop_op /=.
+          destruct (decide _); destruct (repeat () (length σ_f) !! i) as [ [] | ] eqn:Hlook; rewrite Hlook /= //.
+          apply lookup_lt_Some in Hlook.
+          rewrite repeat_length in Hlook.
+          lia.
+      + iIntros (σ_c v_c) "!> R %HorderPC %HorderCF".
+        (* we pick [t] to be [excl_ops_trans (length σ_c)] *)
+        iMod (ops_token_strengthen (length σ_c) with "ops_token") as "[ops_token _]".
+        { by apply prefix_length. }
+        iMod (token_pick (DS := [#]) _ [#] _ _ [##]%HV (excl_ops_trans (length σ_c)) with "[] ops_token") as "[token picked_out]".
+        { by eexists. }
+        { iIntros (i'). inversion i'. }
+        iModIntro.
+        destruct (last σ_c) as [[ w | ] | ]; iModIntro.
+        * iDestruct "ops_auth" as (?) "[picked_in ops_auth]".
+          iPickedInAgree "picked_out picked_in".
+          iDestruct "R" as "[% R]".
+          iFrame "∗%".
+          rewrite /excl_ops_trans map_entry_lift_gmap_view_auth /=.
+          iAssert ⎡ ops_auth γ (length σ_c) ⎤%I with "[ops_auth]" as "ops_auth".
+          { iApply (gen_own_proper with "ops_auth").
+            f_equiv.
+            rewrite map_equiv_iff.
+            intros i.
+            rewrite map_lookup_imap ?lookup_map_seq_0 /drop_op /=.
+            destruct (decide _);
+              destruct (repeat () (length σ_f) !! i) as [ [] | ] eqn:Hlook1;
+              destruct (repeat () (length σ_c) !! i) as [ [] | ] eqn:Hlook2;
+              rewrite ?Hlook1 ?Hlook2 /= //.
+            - apply lookup_ge_None in Hlook2.
+              rewrite repeat_length in Hlook2. 
+              lia.
+            - apply lookup_ge_None in Hlook1.
+              rewrite repeat_length in Hlook1.
+              assert (length σ_c ≤ length σ_f) by by apply prefix_length. 
+              lia.
+            - apply lookup_lt_Some in Hlook2.
+              rewrite repeat_length in Hlook2. 
+              lia.
+            - apply lookup_lt_Some in Hlook2.
+              rewrite repeat_length in Hlook2. 
+              lia. }
+          iDestruct "R" as "[ $ [ $ | ops_frag ]]"; first done.
+          iDestruct (ops_auth_ops_frag_false with "ops_auth ops_frag") as %[].
+        * iDestruct "ops_auth" as (?) "[picked_in ops_auth]".
+          iPickedInAgree "picked_out picked_in".
+          iDestruct "R" as "%".
+          iFrame "∗%".
+          rewrite /excl_ops_trans map_entry_lift_gmap_view_auth /=.
+          iAssert ⎡ ops_auth γ (length σ_c) ⎤%I with "[ops_auth]" as "$".
+          { iApply (gen_own_proper with "ops_auth").
+            f_equiv.
+            rewrite map_equiv_iff.
+            intros i.
+            rewrite map_lookup_imap ?lookup_map_seq_0 /drop_op /=.
+            destruct (decide _);
+              destruct (repeat () (length σ_f) !! i) as [ [] | ] eqn:Hlook1;
+              destruct (repeat () (length σ_c) !! i) as [ [] | ] eqn:Hlook2;
+              rewrite ?Hlook1 ?Hlook2 /= //.
+            - apply lookup_ge_None in Hlook2.
+              rewrite repeat_length in Hlook2. 
+              lia.
+            - apply lookup_ge_None in Hlook1.
+              rewrite repeat_length in Hlook1.
+              assert (length σ_c ≤ length σ_f) by by apply prefix_length. 
+              lia.
+            - apply lookup_lt_Some in Hlook2.
+              rewrite repeat_length in Hlook2. 
+              lia.
+            - apply lookup_lt_Some in Hlook2.
+              rewrite repeat_length in Hlook2. 
+              lia. }
+        * iDestruct "ops_auth" as (?) "[picked_in ops_auth]".
+          iPickedInAgree "picked_out picked_in".
+          iDestruct "R" as "%".
+          iFrame "∗%".
+          rewrite /excl_ops_trans map_entry_lift_gmap_view_auth /=.
+          iAssert ⎡ ops_auth γ (length σ_c) ⎤%I with "[ops_auth]" as "$".
+          { iApply (gen_own_proper with "ops_auth").
+            f_equiv.
+            rewrite map_equiv_iff.
+            intros i.
+            rewrite map_lookup_imap ?lookup_map_seq_0 /drop_op /=.
+            destruct (decide _);
+              destruct (repeat () (length σ_f) !! i) as [ [] | ] eqn:Hlook1;
+              destruct (repeat () (length σ_c) !! i) as [ [] | ] eqn:Hlook2;
+              rewrite ?Hlook1 ?Hlook2 /= //.
+            - apply lookup_ge_None in Hlook2.
+              rewrite repeat_length in Hlook2. 
+              lia.
+            - apply lookup_ge_None in Hlook1.
+              rewrite repeat_length in Hlook1.
+              assert (length σ_c ≤ length σ_f) by by apply prefix_length. 
+              lia.
+            - apply lookup_lt_Some in Hlook2.
+              rewrite repeat_length in Hlook2. 
+              lia.
+            - apply lookup_lt_Some in Hlook2.
+              rewrite repeat_length in Hlook2. 
+              lia. }
+    - rewrite /prot /p_read /=.
+      iIntros (σ v) "R".
+      destruct (last σ) as [[ w | ] | ]; iModIntro; done.
+  Qed.
+End Protocol.
+
+Section Proof.
+  Context `{!excl_opsG Σ Ω, !nvmBaseGS Σ Ω, !nvmHighGS Σ Ω, !PerennialG Σ}.
+  Variables (γ: gname) (R: val → dProp Σ).
+  Hypothesis (R_buffer_free: ∀ v, BufferFree (R v)).
+  Hypothesis (R_NGF: ∀ v, IntoNGFlush (R v) (R v)).
+  
+  Definition is_stack ℓ: dProp Σ :=
+    ∃ σs σ_i, ℓ ↦_AT^{prot γ R} (σs ++ [σ_i]).
+
+  #[export] Instance is_stack_persistent ℓ:
+    Persistent (is_stack ℓ).
+  Proof.
+    rewrite /is_stack.
+    apply bi.exist_persistent. intros.
+    apply bi.exist_persistent. intros.
+    apply _.
+  Qed.
+    
+  Lemma wp_try_push ℓ w:
+    val_is_unboxed (SOMEV w) →
+    {{{ is_stack ℓ ∗ R w }}}
+      try_push #ℓ w
+    {{{ RET #(); True }}}.
+  Proof.
+    rewrite /try_push.
+    iIntros (??) "[(%σs & %σ_i & is_stack) R] HΦ".
+    wp_pures.
+    wp_bind (CmpXchg _ _ _).
+    iApply (wp_cmpxchg_at
+              (λ _ _, True%I) (λ _, True%I) True%I
+              (λ _, True%I) (λ σ, ⎡ ops_auth γ (length σ) ⎤)%I with "[$is_stack R]").
+    { iIntros.
+      iSplitR. { iIntros "_". iPureIntro. left. done. }
+      iSplitL.
+      - iIntros.
+        iExists (σ_l ++ [inl w]).
+        iSplitR.
+        { iIntros "!> _".
+          iPureIntro.
+          by apply prefix_app_r. }
+        iSplitR.
+        { iIntros (???) "[ops_auth1 _] [[ops_auth2 _] | [ _ (% & % & % & [ops_auth2 _ ]) ] ]";
+            iDestruct (gen_own_valid_2 with "ops_auth1 ops_auth2") as %[]%gmap_view_auth_op_valid. }
+        iSplitR.
+        { iIntros "!> predP".
+          iSplitR; first by iModIntro.
+          naive_solver. }
+        iSplitR.
+        { iModIntro.
+          iIntros "[[$ R] _]".
+          rewrite /prot /p_read /=.
+          destruct (last σ_l) as [[] | ]; try done.
+          iDestruct "R" as "($ & $ & R)".
+          by iLeft. }
+        iIntros "ops_auth".
+        iMod (ops_auth_grow with "ops_auth") as "[ops_auth _]".
+        iModIntro.
+        iSplitL; last (iSplit; [by iModIntro | done]).
+        rewrite /prot /p_full /=.
+        rewrite app_length /= Nat.add_1_r last_snoc.
+        by iFrame.
+      - iSplit; last done.
+        iModIntro.
+        naive_solver. }
+    iIntros "!>" (????) "_".
+    destruct b; wp_pures; iModIntro; iApply "HΦ"; done.
+  Qed.
+
+  Lemma wp_try_pop ℓ:
+    {{{ is_stack ℓ }}}
+      try_pop #ℓ
+    {{{ v, RET v; (∃ w, ⌜ v = SOMEV w ⌝ ∗ R w) ∨ ⌜ v = NONEV ⌝ }}}.
+  Proof.
+    rewrite /try_pop.
+    iIntros (?) "(%σs & %σ_i & #is_stack) HΦ".
+    wp_pures.
+    wp_bind (Load _ _).
+    iDestruct (mapsto_at_drop with "is_stack") as "mapsto".
+    iApply (wp_load_at_simple ℓ _
+              (λ σ v, ⌜ match last σ with | Some (inl w) => v = SOMEV w ∧ val_is_unboxed v | _ => v = NONEV end ⌝)%I
+              with "[$mapsto]").
+    { iIntros "!>" (σ_l v_l ?) "H".
+      rewrite /prot /p_read /=.
+      destruct (last σ_l) as [[] | ]; try naive_solver.
+      iDestruct "H" as "(% & % & $)".
+      done. }
+    iClear (σ_i) "mapsto is_stack".
+    iIntros "!>" (σ_i v_i) "[#is_stack >%HlastOp]".
+    (* TODO: clever way to achieve this? *)
+    destruct (last σ_i) as [[ v | ] | ]; first destruct (HlastOp) as [-> safe]; wp_pures.
+    - wp_bind (CmpXchg _ _ _).
+      iEval (rewrite -(app_nil_l [σ_i])) in "is_stack".
+      iApply (wp_cmpxchg_at
+                (λ σ_l σ_t, (⎡ gen_own γ (gmap_view_frag (length σ_l) (DfracOwn 1) ()) ⎤ ∗ ⌜ last σ_l = Some (inl v) ⌝ ∗ ⌜ length σ_l < length σ_t ⌝)%I)
+                (λ _, True%I)
+                True%I
+                (λ _, True%I)
+                (λ σ_l, ⎡ ops_auth γ (length σ_l) ⎤ ∗ ⌜ last σ_l = Some (inl v) ⌝)%I with "[$is_stack]").
+      { iIntros.
+        iSplitR. { iIntros "_". iPureIntro. left. done. }
+        iSplit.
+        - iIntros.
+          subst v_l.
+          iExists (σ_l ++ [inr ()]).
+          iSplitR.
+          { iIntros "!> _".
+            iPureIntro.
+            by apply prefix_app_r. }
+          iSplitL.
+          { iIntros (???) "[ops_auth1 _] [[ops_auth2 _] | [ _ (% & % & % & [ops_auth2 _ ]) ] ]";
+              iDestruct (gen_own_valid_2 with "ops_auth1 ops_auth2") as %[]%gmap_view_auth_op_valid. }
+          iSplitL.
+          { iIntros "!> predP".
+            iSplitR; first by iModIntro.
+            naive_solver. }
+          iSplitL.
+          { iModIntro.
+            iIntros "[[$ R] _]".
+            rewrite /prot /p_read /=.
+            destruct (last σ_l) as [[] | ]; try (iDestruct "R" as "%"; congruence).
+            iDestruct "R" as "(%eq & %safe' & R)".
+            injection eq as ->.
+            iSplitL; last done.
+            iSplitR; first done.
+            iSplitPure; first done.
+            iLeft. done. }
+          iIntros "[ops_auth %]".
+          iMod (ops_auth_grow with "ops_auth") as "[ops_auth ops_frag]".
+          iModIntro.
+          iSplitL "ops_auth". 
+          + rewrite /prot /p_full /=.
+            rewrite app_length /= Nat.add_1_r last_snoc.
+            by iFrame.
+          + iFrame.
+            iSplit; first by iModIntro.
+            iSplit; first done.
+            iPureIntro.
+            rewrite app_length /=.
+            lia.
+        - iSplit; last done.
+          iModIntro.
+          naive_solver. }
+      iIntros "!>" (????) "Hpost".
+      destruct b; wp_pures.
+      + iDestruct "Hpost" as "[(_ & >[frag [%Hlook %]] & #is_stack' & seen_state) | [% ?]]"; last done.
+        wp_bind (Flush _).
+        iApply (wp_flush_xchg _ (prot γ R) σ_l σ_t _ _ (R v) with "[is_stack $seen_state frag]").
+        { iDestruct (mapsto_at_store_lb with "is_stack'") as "$".
+          iSplitR; first by iNamed "is_stack".
+          rewrite /exchange_1 /exchange_2 /exchange_3.
+          iIntros (v_t) "!> predR".
+          iDestruct (p_read_p_pure with "predR") as "%".
+          iFrame.
+          iIntros (σ_old v_old) "!>".
+          iSplit.
+          - iIntros (?) "[ops_token _]".
+            rewrite /prot /p_pers /=.
+            iMod (ops_token_strengthen (length σ_t) with "ops_token") as "[$ #rely]".
+            { by apply prefix_length. }
+            iModIntro.
+            iSplitPure; first done.
+            iIntros (?) "!> predR".
+            iModIntro.
+            rewrite /p_read /= Hlook.
+            Transparent ops_frag.
+            iDestruct "predR" as "($ & $ & [$ | [frag' _ ] ] )".
+            + iRight.
+              rewrite /ops_frag.
+              iFrame.
+              iExists _. iFrame "#".
+              done.
+            + iDestruct (gen_own_valid_2 with "frag frag'") as %[contra _]%gmap_view_frag_op_valid.
+              done.
+          - iIntros (?) "[ops_token $]".
+            iDestruct (token_to_rely with "ops_token") as "#rely".
+            iDestruct (rely_to_rely_self with "rely") as "rely_self".
+            iFrame "ops_token".
+            iModIntro.
+            iIntros (?) "!> predR".
+            iModIntro.
+            rewrite /prot /p_read /= Hlook.
+            Transparent ops_frag.
+            iDestruct "predR" as "($ & $ & [$ | [frag' _ ] ])".
+            + iRight.
+              rewrite /ops_frag.
+              iFrame.
+              iExists _. iFrame "#".
+              iPureIntro.
+              eapply Nat.lt_le_trans; first done.
+              by apply prefix_length.
+            + iDestruct (gen_own_valid_2 with "frag frag'") as %[contra _]%gmap_view_frag_op_valid.
+              done. }
+        iIntros "!> R".
+        wp_pures.
+        wp_bind FenceSync.
+        iApply (wp_fence_sync' with "R").
+        iIntros "!> [_ R]".
+        wp_pures.
+        iModIntro.
+        iApply "HΦ".
+        iLeft.
+        iExists v.
+        by iFrame.
+      + iModIntro.
+        iApply "HΦ".
+        by iRight.
+    - subst v_i.
+      wp_pures.
+      iModIntro.
+      iApply "HΦ".
+      by iRight.
+    - subst v_i.
+      wp_pures.
+      iModIntro.
+      iApply "HΦ".
+      by iRight.
+  Qed.
+End Proof.
